src/Primitive/Int/VstEnc.v
@@ -5,17 +5,13 @@ Require Import Clight.dummy Clight.INTEGER Prim.Der_encode_primitive.
 
 Instance CompSpecs : compspecs. Proof. make_compspecs prog. Defined.
 Definition Vprog : varspecs. Proof. mk_varspecs prog. Defined.
-
+ 
 Section Integer_der_encode.
 
-Definition prim_type_s := (Tstruct _ASN__PRIMITIVE_TYPE_s noattr).
-Definition mk_prim_type_s (buf_p : val) size := (buf_p, Vint (Int.repr size)).
-
-
-Definition int_enc_rval td li struct_len buf_size td_p sptr_p := 
+Definition int_enc_rval td li struct_len buf_size td_p st_p := 
   match evalErrW (int_encoder td struct_len buf_size li) [] with
   | Some v => mk_enc_rval (v) Vzero Vzero
-  | None => mk_enc_rval (-1) td_p sptr_p
+  | None => mk_enc_rval (-1) td_p st_p
   end.
 
 Definition int_enc_res td struct_len buf_size li := 
@@ -46,65 +42,79 @@ Proof. make_cs_preserve Der_encode_primitive.CompSpecs CompSpecs. Defined.
 Definition int_der_encode_spec : ident * funspec :=
   DECLARE _INTEGER_encode_der
     WITH res_p : val,  
-         sptr_p : val, sptr_buf : val, tag_b : block, tag_ofs : ptrofs, 
+         st_p : val, sptr_buf : val, tag_b : block, tag_ofs : ptrofs, 
          struct_len : Z, data : list byte,
          td_p : val, td : TYPE_descriptor,
          tag_mode : Z,
          cb_p : val, app_key_p : val
     PRE [tptr enc_rval_s, tptr type_descriptor_s, tptr tvoid, tint, tuint, 
           tptr cb_type, tptr tvoid]
-      PROP (1 = Zlength (tags td);
-            tag_mode = 0;
-            0 <= struct_len <= Int.max_signed - 11;
-            sptr_p <> nullval; 
-            is_pointer_or_null sptr_buf;
-            struct_len = Zlength data;
+      PROP (1 = Zlength (tags td); tag_mode = 0;
+            0 <= struct_len <= Int.max_signed - 11; st_p <> nullval; 
+            is_pointer_or_null sptr_buf; struct_len = Zlength data;
             0 <= Z_of_val sptr_buf + struct_len <= Ptrofs.max_unsigned)
-      PARAMS (res_p; td_p; sptr_p; Vint (Int.repr tag_mode);
+      PARAMS (res_p; td_p; st_p; Vint (Int.repr tag_mode);
               Vint (Int.repr 0); cb_p; app_key_p)
       GLOBALS ()
       SEP (data_at_ Tsh enc_rval_s res_p;
-           field_at Tsh (Tstruct der_encoder._asn_TYPE_descriptor_s noattr) 
-                    (DOT der_encoder._tags) (Vptr tag_b tag_ofs) td_p;
-           field_at Tsh (Tstruct der_encoder._asn_TYPE_descriptor_s noattr)
-                    (DOT der_encoder._tags_count) 
+             
+           (* td *)
+           field_at Tsh (Tstruct _asn_TYPE_descriptor_s noattr) 
+                    (DOT _tags) (Vptr tag_b tag_ofs) td_p;
+           field_at Tsh (Tstruct _asn_TYPE_descriptor_s noattr)
+                    (DOT _tags_count) 
                     (Vint (Int.repr (Zlength (tags td)))) td_p;
            data_at Tsh (tarray tuint (Zlength (tags td))) 
                    (map Vint (map Int.repr (tags td)))
                    (Vptr tag_b tag_ofs);
+           (* st *)
+        (* field_at Tsh prim_type_s (DOT _size) (Vint (Int.repr struct_len)) st_p;
+           field_at Tsh prim_type_s (DOT _buf) sptr_buf st_p; *)
+           data_at Tsh (Tstruct _ASN__PRIMITIVE_TYPE_s noattr)
+                    (sptr_buf, (Vint (Int.repr struct_len))) st_p;
+           
            valid_pointer sptr_buf;
            if eq_dec sptr_buf nullval 
            then emp else
            data_at Tsh (tarray tuchar (Zlength data)) (map Vubyte data) sptr_buf; 
-           field_at Tsh prim_type_s (DOT _size) (Vint (Int.repr struct_len)) sptr_p;
-           field_at Tsh prim_type_s (DOT _buf) sptr_buf sptr_p; 
+           
+           (* cb *)
            data_at_ Tsh enc_key_s app_key_p;
            valid_pointer cb_p; 
            func_ptr' dummy_callback_spec cb_p)
     POST [tvoid]
       PROP ()
       LOCAL ()
-      SEP (field_at Tsh (Tstruct der_encoder._asn_TYPE_descriptor_s noattr) 
-                    (DOT der_encoder._tags) (Vptr tag_b tag_ofs) td_p;
-           field_at Tsh (Tstruct der_encoder._asn_TYPE_descriptor_s noattr)
-                    (DOT der_encoder._tags_count)
+      SEP ((* td *)
+           field_at Tsh (Tstruct _asn_TYPE_descriptor_s noattr) 
+                    (DOT _tags) (Vptr tag_b tag_ofs) td_p;
+           field_at Tsh (Tstruct _asn_TYPE_descriptor_s noattr)
+                    (DOT _tags_count)
                     (Vint (Int.repr (Zlength (tags td)))) td_p;
-           data_at Tsh (tarray tuint (Zlength (tags td)))
+           data_at Tsh (tarray tuchar (Zlength (tags td)))
                    (map Vint (map Int.repr (tags td)))
                    (Vptr tag_b tag_ofs);
-            valid_pointer sptr_buf;
+
+           (* cb *)
+           valid_pointer cb_p;
+           data_at_ Tsh enc_key_s app_key_p;
+           func_ptr' dummy_callback_spec cb_p;
+
+           (* field_at Tsh prim_type_s (DOT _size) (Vint (Int.repr struct_len)) st_p;
+           field_at Tsh prim_type_s (DOT _buf) sptr_buf st_p; *)
+
+           (* st *)
+           data_at Tsh (Tstruct _ASN__PRIMITIVE_TYPE_s noattr)
+                    (sptr_buf, (Vint (Int.repr struct_len))) st_p;
+           valid_pointer sptr_buf;
            if eq_dec sptr_buf nullval 
            then emp else
            data_at Tsh (tarray tuchar (Zlength data)) (map Vubyte data) sptr_buf;
-           field_at Tsh prim_type_s (DOT _size) (Vint (Int.repr struct_len)) sptr_p;
-           field_at Tsh prim_type_s (DOT _buf)  sptr_buf sptr_p;
+           (* result *)
            data_at Tsh enc_rval_s (int_enc_rval td data struct_len 
                                                 (if eq_dec cb_p nullval
                                                 then 0
-                                                else 32) td_p sptr_p) res_p;
-           valid_pointer cb_p;
-           data_at_ Tsh enc_key_s app_key_p;
-           func_ptr' dummy_callback_spec cb_p).
+                                                else 32) td_p st_p) res_p).
 
 Definition Gprog := ltac:(with_library prog [int_der_encode_spec; 
                                                der_primitive_encoder_spec]).
@@ -149,54 +159,68 @@ Proof.
   replace (Tstruct _ASN__PRIMITIVE_TYPE_s noattr) with prim_type_s by reflexivity.
   forward.
   forward_empty_loop.
-  (* add condition about shift here *)
-  forward_if (
+  break_if.
+  Focus 2.
+  (*  sptr_buf <> nullval *)
+  { forward_if (
+      let data_c := canonicalize_int data in
+      let shift' := Zlength data - Zlength data_c in
       PROP ( ) 
-      LOCAL (temp _t'2 sptr_buf; temp _st sptr_p; 
+      LOCAL (temp _t'2 sptr_buf; 
+             temp _st (if eq_dec shift' 0
+                       then st_p
+                       else v_effective_integer); 
              lvar __res__1 enc_rval_s v__res__1;
-           (*  lvar _unconst (Tunion __4050 noattr) v_unconst; *)
              lvar _effective_integer prim_type_s v_effective_integer;
              lvar _rval (Tstruct _asn_enc_rval_s noattr) v_rval; 
              temp __res res_p; temp _td td_p; 
-             temp _sptr sptr_p; temp _tag_mode (Vint (Int.repr tag_mode));
+             temp _sptr st_p; temp _tag_mode (Vint (Int.repr tag_mode));
              temp _tag (Vint (Int.repr 0)); 
              temp _cb cb_p; temp _app_key app_key_p)
-       SEP ((* Local vars *)
-            data_at_ Tsh enc_rval_s v__res__1;
-           (* data_at_ Tsh (Tunion __4050 noattr) v_unconst; *)
-            data_at_ Tsh prim_type_s v_effective_integer;
-            data_at_ Tsh (Tstruct _asn_enc_rval_s noattr) v_rval; 
-            (* type descriptor *)
-            field_at Tsh (Tstruct der_encoder._asn_TYPE_descriptor_s noattr) 
-                    (DOT der_encoder._tags) (Vptr tag_b tag_ofs) td_p;
-           field_at Tsh (Tstruct der_encoder._asn_TYPE_descriptor_s noattr)
-                    (DOT der_encoder._tags_count) (Vint (Int.repr (Zlength (tags td)))) td_p;
-           data_at Tsh (tarray tuint (Zlength (tags td))) (map Vint (map Int.repr (tags td)))
-                   (Vptr tag_b tag_ofs);
-            (* sptr *)
-            valid_pointer sptr_buf;
-            if eq_dec sptr_buf nullval
-            then emp
-            else data_at Tsh (tarray tuchar struct_len) (map Vubyte data) sptr_buf;
-
-            (* st->buf + shift;
-            effective_integer.size = st->size - shift; *)
-            field_at Tsh prim_type_s (DOT _buf) sptr_buf sptr_p;
-            field_at Tsh prim_type_s (DOT _size) (Vint (Int.repr struct_len)) sptr_p; 
-            (* Result *)
+       SEP (data_at_ Tsh enc_rval_s v__res__1;
             data_at_ Tsh enc_rval_s res_p;
-            (* Callback *)
+            data_at_ Tsh (Tstruct _asn_enc_rval_s noattr) v_rval; 
+
+            (* td *)
+            field_at Tsh (Tstruct _asn_TYPE_descriptor_s noattr) 
+                    (DOT _tags) (Vptr tag_b tag_ofs) td_p;
+            field_at Tsh (Tstruct _asn_TYPE_descriptor_s noattr)
+                    (DOT _tags_count) (Vint (Int.repr (Zlength (tags td)))) td_p;
+            data_at Tsh (tarray tuint (Zlength (tags td)))
+                    (map Vint (map Int.repr (tags td))) (Vptr tag_b tag_ofs);
+
+            (* cb *)
             data_at_ Tsh enc_key_s app_key_p;
             valid_pointer cb_p;
-            func_ptr' dummy_callback_spec cb_p)).
+            func_ptr' dummy_callback_spec cb_p;
+
+            (* st *)
+           data_at Tsh (Tstruct _ASN__PRIMITIVE_TYPE_s noattr)
+                    (sptr_buf, (Vint (Int.repr struct_len))) st_p;
+           valid_pointer sptr_buf;
+           if eq_dec sptr_buf nullval 
+           then emp else
+           (data_at Tsh (tarray tuchar shift') (map Vubyte (sublist 0 shift' data)) sptr_buf *
+            data_at Tsh (tarray tuint (Zlength data_c)) (map Vubyte data_c)
+                    (offset_val shift' sptr_buf));                    
+
+           (* st-> buf + shift *)
+          (* valid_pointer (offset_val shift' sptr_buf); *)
+           
+           (* effective_integer *)
+           if eq_dec shift' 0
+           then data_at_ Tsh prim_type_s v_effective_integer
+           else data_at Tsh (Tstruct _ASN__PRIMITIVE_TYPE_s noattr)
+                          (offset_val shift' sptr_buf,
+                           Vint (Int.repr (struct_len - shift')))
+                           v_effective_integer)).
   * (* sptr_buf->buf <> null *)
     destruct sptr_buf; simpl in H;   try contradiction.
     Require Import VstTactics.
-    rewrite if_false by discriminate.
     repeat forward.
     normalize.
     forward_loop (EX z : Z, 
-               PROP (0 <=  z;
+               PROP (0 <= z;
                      Ptrofs.unsigned i + z <= Ptrofs.max_unsigned)
                LOCAL (temp 
                         _end1 
@@ -205,34 +229,31 @@ Proof.
                                  (Ptrofs.add i (Ptrofs.repr struct_len)) (Ptrofs.repr 1))); 
                       temp _buf (Vptr b (Ptrofs.add i (Ptrofs.repr z))); 
                       temp _t'9 (Vint (Int.repr struct_len));
-                      temp _t'2 (Vptr b i); temp _st sptr_p;
+                      temp _t'2 (Vptr b i); temp _st st_p;
                       lvar __res__1 enc_rval_s v__res__1; 
-                    (* lvar _unconst (Tunion __4050 noattr) v_unconst; *)
                       lvar _effective_integer prim_type_s v_effective_integer; 
                       lvar _rval enc_rval_s v_rval; 
                       temp _tag (Vint (Int.repr 0));
-                      temp __res res_p; temp _td td_p; temp _sptr sptr_p;
+                      temp __res res_p; temp _td td_p; temp _sptr st_p;
                       temp _tag_mode (Vint (Int.repr tag_mode));
                       temp _cb cb_p; temp _app_key app_key_p)
                SEP (data_at_ Tsh enc_rval_s v__res__1; 
-                   (* data_at_ Tsh (Tunion __4050 noattr) v_unconst; *)
                     data_at_ Tsh prim_type_s v_effective_integer; 
                     data_at_ Tsh enc_rval_s v_rval;
                     data_at_ Tsh enc_rval_s res_p;
                     data_at_ Tsh enc_key_s app_key_p;
-                     field_at Tsh (Tstruct der_encoder._asn_TYPE_descriptor_s noattr) 
-                              (DOT der_encoder._tags) (Vptr tag_b tag_ofs) td_p;
-                     field_at Tsh (Tstruct der_encoder._asn_TYPE_descriptor_s noattr)
-                              (DOT der_encoder._tags_count) 
+                     field_at Tsh (Tstruct _asn_TYPE_descriptor_s noattr) 
+                              (DOT _tags) (Vptr tag_b tag_ofs) td_p;
+                     field_at Tsh (Tstruct _asn_TYPE_descriptor_s noattr)
+                              (DOT _tags_count) 
                               (Vint (Int.repr (Zlength (tags td)))) td_p;
                      data_at Tsh (tarray tuint (Zlength (tags td)))
                              (map Vint (map Int.repr (tags td)))
                              (Vptr tag_b tag_ofs);
-                     (* sptr *)
                      valid_pointer (Vptr b i);
                       data_at Tsh (tarray tuchar (Zlength data)) (map Vubyte data) (Vptr b i);
-                     field_at Tsh prim_type_s (DOT _buf) (Vptr b i) sptr_p;
-                     field_at Tsh prim_type_s (DOT _size) (Vint (Int.repr struct_len)) sptr_p;  
+                     data_at Tsh (Tstruct _ASN__PRIMITIVE_TYPE_s noattr)
+                    (Vptr b i, (Vint (Int.repr struct_len))) st_p;  
                      valid_pointer cb_p;
                      func_ptr' dummy_callback_spec cb_p))%assert
       continue: (EX z : Z, 
@@ -245,24 +266,22 @@ Proof.
                                  (Ptrofs.add i(Ptrofs.repr struct_len)) (Ptrofs.repr 1))); 
                       temp _t'9 (Vint (Int.repr struct_len));
                       temp _buf (Vptr b(Ptrofs.add i (Ptrofs.repr z))); 
-                      temp _t'2 (Vptr b i); temp _st sptr_p;
+                      temp _t'2 (Vptr b i); temp _st st_p;
                       lvar __res__1 enc_rval_s v__res__1; 
-                     (* lvar _unconst (Tunion __4050 noattr) v_unconst; *)
                       lvar _effective_integer prim_type_s v_effective_integer; 
                       lvar _rval enc_rval_s v_rval; temp _tag (Vint (Int.repr 0));
-                      temp __res res_p; temp _td td_p; temp _sptr sptr_p;
+                      temp __res res_p; temp _td td_p; temp _sptr st_p;
                       temp _tag_mode (Vint (Int.repr tag_mode));
                       temp _cb cb_p; temp _app_key app_key_p)
                SEP (data_at_ Tsh enc_rval_s v__res__1; 
-                   (* data_at_ Tsh (Tunion __4050 noattr) v_unconst; *)
                     data_at_ Tsh prim_type_s v_effective_integer; 
                     data_at_ Tsh enc_rval_s v_rval;
                     data_at_ Tsh enc_rval_s res_p;
                     data_at_ Tsh enc_key_s app_key_p;
-                     field_at Tsh (Tstruct der_encoder._asn_TYPE_descriptor_s noattr) 
-                              (DOT der_encoder._tags) (Vptr tag_b tag_ofs) td_p;
-                     field_at Tsh (Tstruct der_encoder._asn_TYPE_descriptor_s noattr)
-                              (DOT der_encoder._tags_count) 
+                     field_at Tsh (Tstruct _asn_TYPE_descriptor_s noattr) 
+                              (DOT _tags) (Vptr tag_b tag_ofs) td_p;
+                     field_at Tsh (Tstruct _asn_TYPE_descriptor_s noattr)
+                              (DOT _tags_count) 
                               (Vint (Int.repr (Zlength (tags td)))) td_p;
                      data_at Tsh (tarray tuint (Zlength (tags td)))
                              (map Vint (map Int.repr (tags td)))
@@ -270,54 +289,54 @@ Proof.
                      (* sptr *)
                      valid_pointer (Vptr b i);
                       data_at Tsh (tarray tuchar (Zlength data)) (map Vubyte data) (Vptr b i);
-                     field_at Tsh prim_type_s (DOT _buf) (Vptr b i) sptr_p;
-                     field_at Tsh prim_type_s (DOT _size) (Vint (Int.repr struct_len)) sptr_p;  
+                     data_at Tsh (Tstruct _ASN__PRIMITIVE_TYPE_s noattr)
+                    (Vptr b i, (Vint (Int.repr struct_len))) st_p;  
                      valid_pointer cb_p;
                      func_ptr' dummy_callback_spec cb_p))%assert
       break: (EX z : Z,
-              PROP ()
+              PROP (z = Zlength data - Zlength (canonicalize_int data);
+                    0 <= Ptrofs.unsigned i + z <= Ptrofs.max_unsigned;
+                    0 <= z)
               LOCAL (
                      temp 
                        _end1 
                        (Vptr b
                              (Ptrofs.sub 
-                                (Ptrofs.add i(Ptrofs.repr struct_len)) (Ptrofs.repr 1))); 
+                                (Ptrofs.add i (Ptrofs.repr struct_len)) (Ptrofs.repr 1))); 
                      temp _t'9 (Vint (Int.repr struct_len));
-                     temp _buf (Vptr b(Ptrofs.add i(Ptrofs.repr z))); 
+                     temp _buf (Vptr b (Ptrofs.add i (Ptrofs.repr z))); 
                      temp _t'2 (Vptr b i); 
-                     temp _st sptr_p; lvar __res__1 enc_rval_s v__res__1; 
-                    (* lvar _unconst (Tunion __4050 noattr) v_unconst; *)
+                     temp _st st_p; lvar __res__1 enc_rval_s v__res__1; 
                      lvar _effective_integer prim_type_s v_effective_integer; 
                      lvar _rval enc_rval_s v_rval; temp _tag (Vint (Int.repr 0));
-                     temp __res res_p; temp _td td_p; temp _sptr sptr_p;
+                     temp __res res_p; temp _td td_p; temp _sptr st_p;
                      temp _tag_mode (Vint (Int.repr tag_mode));
                      temp _cb cb_p; temp _app_key app_key_p)
               SEP (data_at_ Tsh enc_rval_s v__res__1; 
-                  (*  data_at_ Tsh (Tunion __4050 noattr) v_unconst; *)
                     data_at_ Tsh prim_type_s v_effective_integer; 
                     data_at_ Tsh enc_rval_s v_rval;
                     data_at_ Tsh enc_rval_s res_p;
                     data_at_ Tsh enc_key_s app_key_p;
-                     field_at Tsh (Tstruct der_encoder._asn_TYPE_descriptor_s noattr) 
-                              (DOT der_encoder._tags) (Vptr tag_b tag_ofs) td_p;
-                     field_at Tsh (Tstruct der_encoder._asn_TYPE_descriptor_s noattr)
-                              (DOT der_encoder._tags_count) 
+                     field_at Tsh (Tstruct _asn_TYPE_descriptor_s noattr) 
+                              (DOT _tags) (Vptr tag_b tag_ofs) td_p;
+                     field_at Tsh (Tstruct _asn_TYPE_descriptor_s noattr)
+                              (DOT _tags_count) 
                               (Vint (Int.repr (Zlength (tags td)))) td_p;
                      data_at Tsh (tarray tuint (Zlength (tags td)))
                              (map Vint (map Int.repr (tags td)))
                              (Vptr tag_b tag_ofs);
                      (* sptr *)
                      valid_pointer (Vptr b i);
-                      data_at Tsh (tarray tuchar (Zlength data)) (map Vubyte data) (Vptr b i);
-                     field_at Tsh prim_type_s (DOT _buf) (Vptr b i) sptr_p;
-                     field_at Tsh prim_type_s (DOT _size) (Vint (Int.repr struct_len)) sptr_p;  
+                     data_at Tsh (tarray tuchar (Zlength data)) (map Vubyte data) (Vptr b i);
+                     data_at Tsh (Tstruct _ASN__PRIMITIVE_TYPE_s noattr)
+                             (Vptr b i, (Vint (Int.repr struct_len))) st_p;  
                      valid_pointer cb_p;
                      func_ptr' dummy_callback_spec cb_p))%assert.
-    - (* invariant check *)
+      (* invariant check *)
       Exists 0.
       entailer!.
-    - (* loop *)
-      Intros z.
+      (* loop *)
+    { Intros z.
       forward_if.
       unfold test_order_ptrs, sameblock.
       destruct peq; try congruence. simpl.
@@ -378,49 +397,38 @@ Proof.
         pose proof unsigned_repr_le (Byte.unsigned (Znth z data)) T1.
         lia. }
       rewrite Znth_map_Vubyte by lia.
+      (* Switch *)
       forward_if (
           PROP ( ) 
-          LOCAL ((*if eq_dec (Byte.unsigned (Znth z data)) 0 
-                 then temp _t'8 (Vubyte (Znth (z + 1) data))
-                 else if eq_dec (Byte.unsigned (Znth z data)) 255 
-                      then     temp _t'7 (Vubyte (Znth (z + 1) data))
-                      else temp _t'6 (Vubyte (Znth z data)); *)
-                 temp _t'6 (Vubyte (Znth z data)); 
+          LOCAL (temp _t'6 (Vubyte (Znth z data)); 
                  temp _end1 (Vptr b(Ptrofs.sub 
-                                           (Ptrofs.add i(Ptrofs.repr struct_len)) 
+                                           (Ptrofs.add i (Ptrofs.repr struct_len)) 
                                            (Ptrofs.repr 1)));
                  temp _buf (Vptr b (Ptrofs.add i (Ptrofs.repr z)));
                  temp _t'9 (Vint (Int.repr struct_len)); temp _t'2 (Vptr b i); 
-                 temp _st sptr_p; lvar __res__1 enc_rval_s v__res__1;
-                (* lvar _unconst (Tunion __4050 noattr) v_unconst; *)
+                 temp _st st_p; lvar __res__1 enc_rval_s v__res__1;
                  lvar _effective_integer prim_type_s v_effective_integer; 
                  lvar _rval enc_rval_s v_rval;
                  temp _tag (Vint (Int.repr 0)); temp __res res_p; temp _td td_p; 
-                 temp _sptr sptr_p; temp _tag_mode (Vint (Int.repr tag_mode)); 
+                 temp _sptr st_p; temp _tag_mode (Vint (Int.repr tag_mode)); 
                  temp _cb cb_p; temp _app_key app_key_p)
           SEP (data_at_ Tsh enc_rval_s v__res__1; 
-              (* data_at_ Tsh (Tunion __4050 noattr) v_unconst; *)
                data_at_ Tsh prim_type_s v_effective_integer; 
-               data_at_ Tsh enc_rval_s v_rval; 
-               data_at_ Tsh enc_rval_s res_p; 
-
-               field_at Tsh (Tstruct der_encoder._asn_TYPE_descriptor_s noattr) 
-                              (DOT der_encoder._tags) (Vptr tag_b tag_ofs) td_p;
-                     field_at Tsh (Tstruct der_encoder._asn_TYPE_descriptor_s noattr)
-                              (DOT der_encoder._tags_count) 
-                              (Vint (Int.repr (Zlength (tags td)))) td_p;
-                     data_at Tsh (tarray tuint (Zlength (tags td)))
-                             (map Vint (map Int.repr (tags td)))
-                             (Vptr tag_b tag_ofs);
-               
-               data_at_ Tsh enc_key_s app_key_p; 
-
-               valid_pointer (Vptr b i); 
-               
-               data_at Tsh (Tarray tuchar (Zlength data) noattr) (map Vubyte data) 
-                       (Vptr b i); 
-               field_at Tsh prim_type_s (DOT _buf) (Vptr b i) sptr_p; 
-               field_at Tsh prim_type_s (DOT _size) (Vint (Int.repr struct_len)) sptr_p; 
+               data_at_ Tsh enc_rval_s v_rval;
+               data_at_ Tsh enc_rval_s res_p;
+               data_at_ Tsh enc_key_s app_key_p;
+               field_at Tsh (Tstruct _asn_TYPE_descriptor_s noattr) 
+                        (DOT _tags) (Vptr tag_b tag_ofs) td_p;
+               field_at Tsh (Tstruct _asn_TYPE_descriptor_s noattr)
+                        (DOT _tags_count) 
+                        (Vint (Int.repr (Zlength (tags td)))) td_p;
+               data_at Tsh (tarray tuint (Zlength (tags td)))
+                       (map Vint (map Int.repr (tags td)))
+                       (Vptr tag_b tag_ofs);
+               valid_pointer (Vptr b i);
+               data_at Tsh (tarray tuchar (Zlength data)) (map Vubyte data) (Vptr b i);
+               data_at Tsh (Tstruct _ASN__PRIMITIVE_TYPE_s noattr)
+                       (Vptr b i, (Vint (Int.repr struct_len))) st_p;  
                valid_pointer cb_p;
                func_ptr' dummy_callback_spec cb_p)).
       -- (* case 0 *)
@@ -455,7 +463,7 @@ Proof.
           forward.
           Exists z.
           entailer!.
-      }
+               }
       -- (* case 1 *)
       { (* *buf = 255 -> second switch case *)
 
@@ -497,12 +505,15 @@ Proof.
         forward. 
         Exists z.
         entailer!.
+        (* z = Zlength data - Zlength (canonicalize_int data) *)
+        admit.
+    }
     - (* continue post-condition *)
       Intros z.
       forward.
       Exists (z + 1).
       entailer!. 
-    - (* after switch shift manipulation *)
+      - (* after switch shift' manipulation *)
       Intros z.
       repeat forward.
       entailer!.
@@ -510,27 +521,67 @@ Proof.
       unfold sameblock.
       destruct peq; try congruence.
       entailer!.
-      forward_if.
-      + (* shift <> 0 *)
-        (*
+      assert (force_val
+                (sem_binary_operation' Osub (tptr tuchar) (tptr tuchar)
+                                       (Vptr b (Ptrofs.add i (Ptrofs.repr z))) (Vptr b i))
+              = Vint (Int.repr z)) as V.
+      { cbn. 
+        unfold sem_sub.
+        cbn. rewrite_if_b. cbn.
+        erewrite Ptrofs.divs_one.
+        unfold Ptrofs.sub.
+        unfold Ptrofs.add.  
+        strip_repr.
+        repeat erewrite Ptrofs.unsigned_repr.
+        repeat f_equal.
+        lia.
+        all: try rep_omega. }
+      erewrite V.
+      forward_if.        
+      + (* shift' <> 0 *)
         repeat forward.
+        erewrite <- H6.
+        repeat rewrite_if_b.
+        unfold offset_val.
+        unfold prim_type_s.
+        unfold asn_codecs_prim._ASN__PRIMITIVE_TYPE_s.        
         entailer!.
-        (* sptr_p = v_effective_integer WHY ?*)
+        remember (Zlength data - Zlength (canonicalize_int data)) as z.
+        Require Import SepLemmas.
+        erewrite data_at_app_gen        
+          with (j1 := z) (ls1 := (map Vubyte (sublist 0 z data)))
+        (j2 := Zlength (canonicalize_int data)) 
+        (ls2 := (map Vubyte (canonicalize_int data))).
+        entailer!.
+        admit. (* tuchar tuint issue *)
+        all: try erewrite Zlength_map.
+        all: try list_solve.
+        subst.
+        erewrite <- map_app.
+        f_equal.
+        autorewrite with sublist.
+        (* data = sublist 0 (Zlength data -
+           Zlength (canonicalize_int data)) data ++ canonicalize_int dat *)
         admit.
-        rewrite if_false by discriminate.
-        entailer!.
-      + (* shift = 0 *)
+        autorewrite with sublist.
+        subst. 
+        admit.
+      + (* shift' = 0 *)
         forward.
-        rewrite if_false by discriminate.
-        entailer!. 
-  * (* sptr_buf = nullval *)
-    forward.
-    subst.
-    repeat rewrite if_true by auto.
-    entailer!.
+        erewrite <- H6.
+        repeat rewrite_if_b.
+        rewrite if_true.
+        repeat rewrite_if_b.
+        rewrite if_true.
+        entailer!.
+        erewrite data_at_app_gen.
+        entailer!.
+        all: admit.  (* z = 0 *)
+  * congruence.
   * (* sptr_buf is null or pointer - we pass it to prim decoder anyway *)
-    forward_call (v__res__1,   
-                  sptr_p,
+    destruct (eq_dec (Zlength data - Zlength (canonicalize_int data)) 0). 
+    ** (* forward_call (v__res__1,   
+                  st_p,
                   tag_b, tag_ofs,
                   sptr_buf, 
                   map Byte.unsigned data,
@@ -538,23 +589,16 @@ Proof.
                   td_p, td,
                   0,
                   cb_p, app_key_p).
-    entailer!.
+    entailer!.    
     unfold Frame.
-    instantiate (1 := [(* data_at_ Tsh (Tunion __4050 noattr) v_unconst * *)
-                       data_at_ Tsh prim_type_s v_effective_integer *
+    rewrite_if_b.
+    instantiate (1 := [data_at_ Tsh prim_type_s v_effective_integer *
                        data_at_ Tsh (Tstruct _asn_enc_rval_s noattr) v_rval *
                        data_at_ Tsh enc_rval_s res_p]).
     simpl.
-    break_if; entailer!.
-    (* compspecs issue *)
-    admit.
-    replace (Zlength (map Byte.unsigned data)) with (Zlength (data)).
-    replace (map Vint (map Int.repr (map Byte.unsigned data))) with (map Vubyte data).
     entailer!.
-    (* tuint and tuchar issue, compspecs issue *)
+    (* compspecs and tuint issue *)
     admit.
-    admit.
-    erewrite Zlength_map. auto.
     Intros.
     unfold prim_enc_rval.
     destruct (evalErrW
@@ -565,7 +609,7 @@ Proof.
        forward_if_add_sep (
         if eq_dec (Vint Int.zero) v_effective_integer 
         then data_at Tsh (Tstruct _asn_enc_rval_s noattr)
-                       (Vint (Int.repr z), (Vint Int.zero, sptr_p))
+                       (Vint (Int.repr z), (Vint Int.zero, st_p))
                        v_rval
         else data_at Tsh (Tstruct _asn_enc_rval_s noattr)
                        (Vint (Int.repr z),
@@ -606,13 +650,13 @@ Proof.
           unfold not; intro K;
           inversion K; contradiction.
        ++ destruct (eq_dec (Vint Int.zero) v_effective_integer) eqn : S.
-          **
+          ***
           repeat forward.
-          **
+          ***
           repeat forward.
           entailer!.
           assert ((int_enc_rval td data (Zlength data) (if eq_dec cb_p nullval then 0 else 32)
-                                td_p sptr_p) = 
+                                td_p st_p) = 
                    (Vint (Int.repr z), (Vint Int.zero, Vint Int.zero))) as RES.
            { unfold int_enc_rval.
              unfold evalErrW.
@@ -641,13 +685,13 @@ Proof.
            admit.
     -- repeat forward.       
        forward_if_add_sep (
-        if eq_dec sptr_p v_effective_integer 
+        if eq_dec st_p v_effective_integer 
         then data_at Tsh (Tstruct _asn_enc_rval_s noattr)
-                     (Vint (Int.repr (-1)), (td_p, sptr_p)) v_rval
+                     (Vint (Int.repr (-1)), (td_p, st_p)) v_rval
         else data_at Tsh (Tstruct _asn_enc_rval_s noattr)
-                     (Vint (Int.repr (-1)), (td_p, sptr_p)) v_rval) v_rval.
+                     (Vint (Int.repr (-1)), (td_p, st_p)) v_rval) v_rval.
        ++ eapply denote_tc_test_eq_split.
-          admit. (* valid_pointer sptr_p *)
+          admit. (* valid_pointer st_p *)
           unfold prim_type_s.
           unfold data_at_.
           unfold field_at_.
@@ -663,11 +707,11 @@ Proof.
           entailer!. 
        ++ forward.
           break_if.
-          ** rewrite if_true.
+          *** rewrite if_true.
              entailer!.
-          { (* need  typed_true tint (force_val (sem_cmp_pp Ceq sptr_p v_effective_integer))
-               ->   sptr_p = v_effective_integer *)  admit. }
-          ** rewrite if_false.
+          { (* need  typed_true tint (force_val (sem_cmp_pp Ceq st_p v_effective_integer))
+               ->   st_p = v_effective_integer *)  admit. }
+          *** rewrite if_false.
              entailer!.
              admit.
        ++ forward.
@@ -676,8 +720,8 @@ Proof.
           admit.
           { admit. }
        ++ 
-         destruct (eq_dec sptr_p v_effective_integer) eqn: EI.
-          **
+         destruct (eq_dec st_p v_effective_integer) eqn: EI.
+          ***
           repeat forward.
           entailer!.
               assert ((int_enc_rval td data (Zlength data) 
@@ -705,14 +749,14 @@ Proof.
            entailer!.
            (* tuint and tuchar issue, compspecs issue *)
            admit.
-          **
+          ***
           repeat forward.
           entailer!.
            assert ((int_enc_rval td data (Zlength data)
                                  (if eq_dec cb_p nullval
                                   then 0 else 32) 
-                                 td_p sptr_p) = 
-                   (Vint (Int.repr (-1)), (td_p, sptr_p))) as RES.
+                                 td_p st_p) = 
+                   (Vint (Int.repr (-1)), (td_p, st_p))) as RES.
            {  unfold int_enc_rval.
               unfold evalErrW.
               unfold int_encoder.
@@ -732,7 +776,232 @@ Proof.
            erewrite RES.
            entailer!.
            (* tuint and tuchar issue, compspecs issue *)
-           admit.  
+           admit. *)
+      admit. 
+    ** forward_call (v__res__1,   
+                  v_effective_integer,
+                  tag_b, tag_ofs,
+                  (offset_val (Zlength data -
+                              Zlength (canonicalize_int data))) sptr_buf, 
+                  map Byte.unsigned (canonicalize_int data),
+                  struct_len - (Zlength data - Zlength (canonicalize_int data)),
+                  td_p, td,
+                  0,
+                  cb_p, app_key_p).
+    entailer!.       
+    unfold Frame.
+    instantiate
+      (1 := [data_at_ Tsh (Tstruct _asn_enc_rval_s noattr) v_rval *
+             data_at_ Tsh enc_rval_s res_p *
+             data_at Tsh (tarray tuchar
+                                 (Zlength data - Zlength (canonicalize_int data)))
+                     (map Vubyte (sublist 0 (Zlength data - Zlength (canonicalize_int data)) data)) 
+                     sptr_buf *
+             data_at Tsh (Tstruct _ASN__PRIMITIVE_TYPE_s noattr)
+                     (sptr_buf, Vint (Int.repr struct_len)) st_p]).
+    destruct sptr_buf; simpl in H3; try contradiction; try discriminate.
+    erewrite H3 in *. contradiction.
+    unfold offset_val.
+    rewrite if_false by discriminate.
+    rewrite if_false by discriminate.
+    simpl.
+    entailer!.
+    remember (Zlength data - Zlength (canonicalize_int data)) as z.
+    (* need  valid_pointer (offset_val shift' sptr_buf)
+       *)
+    (* compspecs issue *)
+    admit.
+    pose proof (can_data_len data). 
+    repeat split; auto; try lia.
+    list_solve.
+    Intros.
+    unfold prim_enc_rval.
+    destruct (evalErrW
+           (Exec.primitive_encoder td (struct_len - 
+                                       (Zlength data - Zlength (canonicalize_int data)))
+                                   (if eq_dec cb_p nullval then 0 else 32)
+                                   (map Int.repr (map Byte.unsigned
+                                                      (canonicalize_int data)))) []) eqn : G.
+    -- repeat forward. 
+       Require Import Forward.
+       forward_if_add_sep (
+        if eq_dec (Vint Int.zero) v_effective_integer 
+        then data_at Tsh (Tstruct _asn_enc_rval_s noattr)
+                       (Vint (Int.repr z), (Vint Int.zero, st_p))
+                       v_rval
+        else data_at Tsh (Tstruct _asn_enc_rval_s noattr)
+                       (Vint (Int.repr z),
+                        (Vint Int.zero, Vint Int.zero)) v_rval) v_rval.
+     (*  ++ entailer!.
+          eapply denote_tc_test_eq_split.
+          entailer!.
+          unfold prim_type_s.
+          unfold data_at_.
+          unfold field_at_.
+          simpl.
+          assert (0 < sizeof (Tstruct _ASN__PRIMITIVE_TYPE_s noattr)) by (cbn; lia).
+          assert (field_at Tsh (Tstruct _ASN__PRIMITIVE_TYPE_s noattr) []
+                           (default_val
+                              (Tstruct _ASN__PRIMITIVE_TYPE_s noattr))
+                           v_effective_integer
+                           |-- valid_pointer v_effective_integer) as F.
+          { eapply field_at_valid_ptr0; cbn; auto.
+            lia. }
+          entailer!.
+          (* valid_pointer v_effective_integer *)
+          admit. *)
+       ++ forward.
+          break_if;
+          rewrite if_true;
+          try entailer!.
+          all: destruct v_effective_integer; cbn in H; try contradiction;
+          try discriminate;
+          eapply typed_true_of_bool in H;
+          eapply int_eq_e in H;
+          erewrite H; auto.
+       ++ forward.
+          break_if;
+          rewrite if_false;
+          try entailer!;
+          destruct v_effective_integer; cbn in H; try contradiction;
+          try discriminate;
+          eapply typed_false_of_bool in H;
+          eapply int_eq_false_e in H;
+          unfold not; intro K;
+          inversion K; contradiction.
+       ++ destruct (eq_dec (Vint Int.zero) v_effective_integer) eqn : S.
+          ***
+          repeat forward.
+          ***
+          repeat forward.
+          entailer!.
+          assert ((int_enc_rval td data 
+                                (Zlength data)
+                                (if eq_dec cb_p nullval 
+                                 then 0 else 32)
+                                td_p st_p) = 
+                   (Vint (Int.repr z), (Vint Int.zero, Vint Int.zero))) as RES.
+           { unfold int_enc_rval.
+             unfold evalErrW.
+             unfold int_encoder.
+             generalize G.
+             break_if.
+             -
+             Require Import VstTactics.
+             rewrite_if_b.
+             unfold evalErrW.
+             break_match. congruence.
+             break_let. intro GG.
+             inversion GG.
+             auto.
+             - rewrite_if_b.
+               unfold evalErrW.
+               break_match. congruence.
+               break_let. intro GG.
+               inversion GG. auto. }
+           erewrite RES.
+           entailer!.
+           destruct sptr_buf; simpl in H3; try contradiction; try discriminate.
+           erewrite H3 in *. contradiction.
+           unfold offset_val.
+           rewrite if_false by discriminate.
+           entailer!.
+           (* data_at_app_gen proof *)
+           admit.
+    -- repeat forward.       
+       forward_if_add_sep (
+        if eq_dec st_p v_effective_integer 
+        then data_at Tsh (Tstruct _asn_enc_rval_s noattr)
+                     (Vint (Int.repr (-1)), (td_p, st_p)) v_rval
+        else data_at Tsh (Tstruct _asn_enc_rval_s noattr)
+                     (Vint (Int.repr (-1)), (td_p, st_p)) v_rval) v_rval.
+      (* ++ eapply denote_tc_test_eq_split.
+          admit. (* valid_pointer st_p *)
+          unfold prim_type_s.
+          unfold data_at_.
+          unfold field_at_.
+          simpl.
+          assert (0 < sizeof (Tstruct _ASN__PRIMITIVE_TYPE_s noattr)) by (cbn; lia).
+          assert (field_at Tsh (Tstruct _ASN__PRIMITIVE_TYPE_s noattr) []
+                           (default_val
+                              (Tstruct _ASN__PRIMITIVE_TYPE_s noattr))
+                           v_effective_integer
+                           |-- valid_pointer v_effective_integer) as F.
+          { eapply field_at_valid_ptr0; cbn; auto.
+            lia. }
+          entailer!. 
+          admit. *)
+       ++ forward.
+          break_if.
+          *** rewrite if_true.
+             entailer!.
+          { (* need  typed_true tint (force_val (sem_cmp_pp Ceq st_p v_effective_integer))
+               ->   st_p = v_effective_integer *)  admit. }
+          *** rewrite if_false.
+             entailer!.
+             admit.
+       ++ forward.
+          break_if.
+          (* contradiction *)
+          admit.
+          { admit. }
+       ++ 
+         destruct (eq_dec st_p v_effective_integer) eqn: EI.
+          ***
+          repeat forward.
+          entailer!.
+              assert ((int_enc_rval td data (Zlength data) 
+                                    (if eq_dec cb_p nullval then 0 else 32) td_p
+                                    v_effective_integer) = 
+                   (Vint (Int.repr (-1)), (td_p, v_effective_integer))) as RES.
+              {  unfold int_enc_rval.
+                 unfold evalErrW.
+                 unfold int_encoder.
+                 generalize G.
+                 break_if.
+                 -
+                   Require Import VstTactics.
+                   rewrite_if_b.
+                   unfold evalErrW.
+                   break_match; try break_let; try congruence.
+                   auto.
+                 - rewrite_if_b.
+                   unfold evalErrW.
+                   break_match;  try break_let; try congruence.
+                   auto.
+           }
+           erewrite RES.
+           entailer!.
+           (* tuint and tuchar issue, compspecs issue *)
+           admit.
+          ***
+          repeat forward.
+          entailer!.
+           assert ((int_enc_rval td data (Zlength data)
+                                 (if eq_dec cb_p nullval
+                                  then 0 else 32) 
+                                 td_p st_p) = 
+                   (Vint (Int.repr (-1)), (td_p, st_p))) as RES.
+           {  unfold int_enc_rval.
+              unfold evalErrW.
+              unfold int_encoder.
+              generalize G.
+              break_if.
+              -
+                Require Import VstTactics.
+                rewrite_if_b.
+                unfold evalErrW.
+                break_match; try break_let; try congruence.
+                auto.
+              - rewrite_if_b.
+                unfold evalErrW.
+                break_match;  try break_let; try congruence.
+                auto. }
+           erewrite RES.
+           entailer!.
+           (* tuint and tuchar issue, compspecs issue *)
+           admit. } 
+    
 Admitted.
 
 End Integer_der_encode.
